finish 0 and 1

src/computability/epsilon_NFA.lean
@@ -1,7 +1,7 @@
 /-
 Copyright (c) 2021 Fox Thomson. All rights reserved.
 Released under Apache 2.0 license as described in the file LICENSE.
-Authors: Fox Thomson
+Authors: Fox Thomson, Yaël Dillies
 -/
 
 import computability.NFA
@@ -15,6 +15,40 @@ which can be followed without reading a character.
 Since this definition allows for automata with infinite states, a `fintype` instance must be
 supplied for true `ε_NFA`'s.
 -/
+
+section move
+variables {α : Type*}
+
+section
+variables [complete_lattice α] {ι : Sort*} {κ : ι → Sort*} {f : Π i, κ i → α}
+
+@[simp] lemma infi₂_eq_top : (⨅ i j, f i j) = ⊤ ↔ ∀ i j, f i j = ⊤ := by simp_rw infi_eq_top
+@[simp] lemma supr₂_eq_bot : (⨆ i j, f i j) = ⊥ ↔ ∀ i j, f i j = ⊥ := by simp_rw supr_eq_bot
+
+end
+
+namespace set
+variables {ι : Sort*} {κ : ι → Sort*} {s : set α}
+
+lemma eq_empty_of_forall_not_mem (h : ∀ x, x ∉ s) : s = ∅ := ext $ λ a, iff_of_false (h _) id
+
+@[simp] lemma Union₂_eq_empty {s : Π i, κ i → set α} : (⋃ i j, s i j) = ∅ ↔ ∀ i j, s i j = ∅ := supr₂_eq_bot
+
+@[simp] lemma Inter₂_eq_univ {s : Π i, κ i → set α} :
+  (⋂ i j, s i j) = univ ↔ ∀ i j, s i j = univ :=
+infi₂_eq_top
+
+@[simp] lemma Union_pos {p : Prop} {s : p → set α} (h : p) : (⋃ i, s i) = s h := supr_pos h
+@[simp] lemma Inter_pos {p : Prop} {s : p → set α} (h : p) : (⋂ i, s i) = s h := infi_pos h
+@[simp] lemma Union_neg' {p : Prop} {s : p → set α} (h : ¬ p) : (⋃ i, s i) = ∅ := supr_neg h
+@[simp] lemma Inter_neg' {p : Prop} {s : p → set α} (h : ¬ p) : (⋂ i, s i) = univ := infi_neg h
+
+end set
+
+lemma option.mem_some (a : α) : a ∈ some a := option.mem_some_iff.2 rfl
+lemma option.mem_coe (a : α) : a ∈ (a : option α) := option.mem_some _
+
+end move
 
 open set
 
@@ -31,117 +65,293 @@ structure ε_NFA (α : Type u) (σ : Type v) :=
 (start : set σ)
 (accept : set σ)
 
-variables {α : Type u} {σ σ' : Type v} (M : ε_NFA α σ)
+variables {α : Type u} {σ σ' : Type v} (M : ε_NFA α σ) {S : set σ} {x : list α} {s : σ} {a : α}
 
 namespace ε_NFA
 
 /-- The `ε_closure` of a set is the set of states which can be reached by taking a finite string of
   ε-transitions from an element of the set -/
-inductive ε_closure : set σ → set σ
-| base : ∀ S (s ∈ S), ε_closure S s
-| step : ∀ S s (t ∈ M.step s none), ε_closure S s → ε_closure S t
+inductive ε_closure (S : set σ) : set σ
+| base : ∀ s ∈ S, ε_closure s
+| step : ∀ s (t ∈ M.step s none), ε_closure s → ε_closure t
+
+@[simp] lemma subset_ε_closure (S : set σ) : S ⊆ M.ε_closure S := ε_closure.base
+
+@[simp] lemma ε_closure_empty : M.ε_closure ∅ = ∅ :=
+eq_empty_of_forall_not_mem $ λ s hs, by induction hs with t ht _ _ _ _ ih; assumption
+
+@[simp] lemma ε_closure_univ : M.ε_closure univ = univ :=
+eq_univ_of_univ_subset $ subset_ε_closure _ _
 
 /-- `M.step_set S a` is the union of the ε-closure of `M.step s a` for all `s ∈ S`. -/
-def step_set : set σ → α → set σ :=
-λ S a, S >>= (λ s, M.ε_closure (M.step s a))
+def step_set (S : set σ) (a : α) : set σ := ⋃ s ∈ S, M.ε_closure $ M.step s a
+
+variables {M}
+
+@[simp] lemma mem_step_set_iff : s ∈ M.step_set S a ↔ ∃ t ∈ S, s ∈ M.ε_closure (M.step t a) :=
+mem_Union₂
+
+@[simp] lemma step_set_empty (a : α) : M.step_set ∅ a = ∅ :=
+by simp_rw [step_set, Union_false, Union_empty]
+
+variables (M)
 
 /-- `M.eval_from S x` computes all possible paths through `M` with input `x` starting at an element
   of `S`. -/
 def eval_from (start : set σ) : list α → set σ :=
 list.foldl M.step_set (M.ε_closure start)
 
+@[simp] lemma eval_from_nil (S : set σ) : M.eval_from S [] = M.ε_closure S := rfl
+@[simp] lemma eval_from_singleton (S : set σ) (a : α) :
+  M.eval_from S [a] = M.step_set (M.ε_closure S) a := rfl
+@[simp] lemma eval_from_append_singleton (S : set σ) (x : list α) (a : α) :
+  M.eval_from S (x ++ [a]) = M.step_set (M.eval_from S x) a :=
+by simp only [eval_from, list.foldl_append, list.foldl_cons, list.foldl_nil]
+
+@[simp] lemma eval_from_empty (x : list α) : M.eval_from ∅ x = ∅ :=
+begin
+  induction x using list.reverse_rec_on with x a ih,
+  { rw [eval_from_nil, ε_closure_empty] },
+  { rw [eval_from_append_singleton, ih, step_set_empty] }
+end
+
 /-- `M.eval x` computes all possible paths through `M` with input `x` starting at an element of
   `M.start`. -/
 def eval := M.eval_from M.start
 
+@[simp] lemma eval_nil : M.eval [] = M.ε_closure M.start := rfl
+@[simp] lemma eval_singleton (a : α) : M.eval [a] = M.step_set (M.ε_closure M.start) a := rfl
+@[simp] lemma eval_append_singleton (x : list α) (a : α) :
+  M.eval (x ++ [a]) = M.step_set (M.eval x) a :=
+eval_from_append_singleton _ _ _ _
+
 /-- `M.accepts` is the language of `x` such that there is an accept state in `M.eval x`. -/
-def accepts : language α :=
-λ x, ∃ S ∈ M.accept, S ∈ M.eval x
+def accepts : language α := {x | ∃ S ∈ M.accept, S ∈ M.eval x}
 
 /-! ### Regex-like operations -/
 
-variables (α σ)
+instance : has_zero (ε_NFA α σ) := ⟨⟨λ _ _, ∅, ∅, ∅⟩⟩
+instance : has_one (ε_NFA α σ) := ⟨⟨λ _ _, ∅, univ, univ⟩⟩
 
-protected def zero : ε_NFA α σ :=
-ε_NFA.mk (λ _ _, ∅) ∅ ∅
+instance : inhabited (ε_NFA α σ) := ⟨0⟩
 
-instance : has_zero (ε_NFA α σ) := ⟨ε_NFA.zero α σ⟩
+variables (P : ε_NFA α σ) (Q : ε_NFA α σ')
 
-protected def one : ε_NFA α σ :=
-{ step := λ _ _, univ,
+/-- Addition of `ε_NFA`s. The language of `P.add Q` is the sum of the languages of `P` and `Q`.
+-/
+def add : ε_NFA α (σ × σ') :=
+{ step := λ s a, P.step s.1 a ×ˢ Q.step s.2 a,
+  start := P.start ×ˢ Q.start,
+  accept := {ab | ab.1 ∈ P.accept ∨ ab.2 ∈ Q.accept} }
+
+/-- Multiplication of `ε_NFA`s. The language of `P.mul Q` is the product of the languages of `P` and
+`Q`. -/
+def mul : ε_NFA α (σ × σ') :=
+{ step := λ s a, P.step s.1 a ×ˢ Q.step s.2 a,
+  start := P.start ×ˢ Q.start,
+  accept := P.accept ×ˢ Q.accept }
+
+def char [decidable_eq α] (a : α) : ε_NFA α (option unit) :=
+{ step := λ s, match s with
+    | none := λ b, if a ∈ b then {some ()} else ∅
+    | some s := λ _, ∅
+    end,
   start := univ,
   accept := univ }
 
-instance : has_one (ε_NFA α σ) := ⟨ε_NFA.one α σ⟩
-
-variables {α σ} (P : ε_NFA α σ) (Q : ε_NFA α σ')
-
-def char [decidable_eq α] (a : α) : ε_NFA α (option unit) :=
-{ step := λ s b, if (a ∈ b ∧ s = none) then {some ()} else ∅,
-    start := set.univ,
-    accept := set.univ }
-
-def add : ε_NFA α (σ × σ') :=
-{ step := λ s a, (P.step s.1 a).prod (Q.step s.2 a),
-  start := P.start.prod Q.start,
-  accept := {ab | ab.1 ∈ P.accept ∨ ab.2 ∈ Q.accept} }
-
-protected def mul : ε_NFA α (σ × σ') :=
-{ step := λ s a, (P.step s.1 a).prod (Q.step s.2 a),
-  start := P.start.prod Q.start,
-  accept := P.accept.prod Q.accept }
-
-
-def star [Π s, decidable (s ∈ P.accept)] : ε_NFA α (option σ) :=
+def star [decidable_pred (∈ P.accept)] : ε_NFA α (option σ) :=
 { step := λ s a, match s with
     | none := match a with
-      | none := coe '' P.start
-      | (some a) := ∅
+      | none := some '' P.start
+      | some a := ∅
       end
-    | (some s) :=  match a with
-      | none := (coe '' P.step s none) ∪ (if (s ∈ P.accept) then {none} else ∅)
-      | (some a) := coe '' P.step s a
+    | some s :=  match a with
+      | none := if s ∈ P.accept then insert none (some '' P.step s none) else some '' P.step s none
+      | some a := some '' P.step s a
       end
     end,
   start := {none},
   accept := {none} }
 
-lemma accept_zero : (0 : ε_NFA α σ).accept = ∅ := rfl
+@[simp] lemma step_zero (s a) : (0 : ε_NFA α σ).step s a = ∅ := rfl
+@[simp] lemma step_one (s a) : (1 : ε_NFA α σ).step s a = ∅ := rfl
+@[simp] lemma step_add (s a) : (P.add Q).step s a = P.step s.1 a ×ˢ Q.step s.2 a := rfl
+@[simp] lemma step_mul (s a) : (P.mul Q).step s a = P.step s.1 a ×ˢ Q.step s.2 a := rfl
 
-lemma accepts_zero : (0 : ε_NFA α σ).accepts = 0 :=
+@[simp] lemma step_char_none_left [decidable_eq α] (a : α) (b : option α) :
+  (char a).step none b = if a ∈ b then {some ()} else ∅ := rfl
+@[simp] lemma step_char_none_some [decidable_eq α] (a : α) :
+  (char a).step none (some a) = {some ()} := if_pos rfl
+@[simp] lemma step_char_some [decidable_eq α] (a : α) (b : option α) (s : unit) :
+  (char a).step (some s) b = ∅ := rfl
+@[simp] lemma step_char_none_right [decidable_eq α] (a : α) :
+  ∀ s : option unit, (char a).step s none = ∅
+| none := by rw [step_char_none_left, if_neg (option.not_mem_none _)]
+| (some s) := rfl
+
+@[simp] lemma step_star_none_none [decidable_pred (∈ P.accept)] :
+  P.star.step none none = some '' P.start := rfl
+@[simp] lemma step_star_none_some [decidable_pred (∈ P.accept)] (a : α) :
+  P.star.step none a = ∅ := rfl
+@[simp] lemma step_star_some_none [decidable_pred (∈ P.accept)] (s : σ) :
+  P.star.step s none =
+    if s ∈ P.accept then insert none (some '' P.step s none) else some '' P.step s none := rfl
+lemma step_star_some_none_of_mem [decidable_pred (∈ P.accept)] {s} (h : s ∈ P.accept) :
+  P.star.step s none = insert none (some '' P.step s none) := if_pos h
+lemma step_star_some_none_of_not_mem [decidable_pred (∈ P.accept)] {s} (h : s ∉ P.accept) :
+  P.star.step s none = some '' P.step s none := if_neg h
+
+@[simp] lemma start_zero : (0 : ε_NFA α σ).start = ∅ := rfl
+@[simp] lemma start_one : (1 : ε_NFA α σ).start = univ := rfl
+@[simp] lemma start_add : (P.add Q).start = P.start ×ˢ Q.start := rfl
+@[simp] lemma start_mul : (P.mul Q).start = P.start ×ˢ Q.start := rfl
+@[simp] lemma start_char [decidable_eq α] (a : α) : (char a).start = univ := rfl
+@[simp] lemma start_star [decidable_pred (∈ P.accept)] : P.star.start = {none} := rfl
+
+@[simp] lemma accept_zero : (0 : ε_NFA α σ).accept = ∅ := rfl
+@[simp] lemma accept_one : (1 : ε_NFA α σ).accept = univ := rfl
+@[simp] lemma accept_add : (P.add Q).accept = {ab | ab.1 ∈ P.accept ∨ ab.2 ∈ Q.accept} := rfl
+@[simp] lemma accept_mul : (P.mul Q).accept = P.accept ×ˢ Q.accept := rfl
+@[simp] lemma accept_char [decidable_eq α] (a : α) : (char a).accept = univ := rfl
+@[simp] lemma accept_star [decidable_pred (∈ P.accept)] : P.star.accept = {none} := rfl
+
+@[simp] lemma ε_closure_zero (S : set σ) : (0 : ε_NFA α σ).ε_closure S = S :=
 begin
-  ext,
-  refine iff_of_false _ (language.not_mem_zero _),
-  rintro ⟨s, h, _⟩,
-  exact set.not_mem_empty _ h,
+  refine (subset_ε_closure _ _).antisymm' _,
+  rintro s (⟨t, ht⟩ | ⟨t, u, h⟩),
+  { exact ht },
+  { exact h.elim }
 end
 
-lemma accepts_one : (1 : ε_NFA α σ).accepts = 1 :=
+@[simp] lemma ε_closure_one (S : set σ) : (1 : ε_NFA α σ).ε_closure S = S :=
+begin
+  refine (subset_ε_closure _ _).antisymm' _,
+  rintro s (⟨t, ht⟩ | ⟨t, u, h⟩),
+  { exact ht },
+  { exact h.elim }
+end
+
+-- @[simp] lemma ε_closure_add (S) : (P.add Q).ε_closure S = {ab | ab.1 ∈ P.accept ∨ ab.2 ∈ Q.accept} := rfl
+-- @[simp] lemma ε_closure_mul (S) : (P.mul Q).ε_closure S = P.accept ×ˢ Q.accept := rfl
+-- @[simp] lemma ε_closure_char [decidable_eq α] (S) (a : α) : (char a).ε_closure S = univ :=
+-- begin
+
+-- end
+-- @[simp] lemma ε_closure_star (S) [decidable_pred (∈ P.accept)] : P.star.ε_closure S = {none} := rfl
+
+@[simp] lemma step_set_zero (S : set σ) (a : α) : (0 : ε_NFA α σ).step_set S a = ∅ :=
+by simp_rw [step_set, step_zero, ε_closure_empty, Union_empty]
+
+@[simp] lemma step_set_one (S : set σ) (a : α) : (1 : ε_NFA α σ).step_set S a = ∅ :=
+by simp_rw [step_set, step_one, ε_closure_empty, Union_empty]
+
+-- @[simp] lemma step_set_add : (P.add Q).step_set S a = {ab | ab.1 ∈ P.accept ∨ ab.2 ∈ Q.accept} := rfl
+-- @[simp] lemma step_set_mul : (P.mul Q).step_set S a = P.accept ×ˢ Q.accept := rfl
+
+lemma step_set_char_of_none_mem [decidable_eq α] {S : set (option unit)} (hS : none ∈ S) (a : α) :
+  (char a).step_set S a = {some ()} :=
+begin
+  unfold step_set,
+  simp only [Union_option, step_char_none_left, step_char_some, ε_closure_empty, Union_empty,
+    union_empty, if_pos (option.mem_coe _), Union_pos hS],
+  refine (subset_ε_closure _ _).antisymm' _,
+  rintro s (⟨_, hs⟩ | ⟨t, ht, hs⟩),
+  { exact hs },
+  { rw  step_char_none_right at hs,
+    exact hs.elim }
+end
+
+lemma step_set_char_of_none_not_mem [decidable_eq α] {S : set (option unit)} (hS : none ∉ S)
+  (a : α) :
+  (char a).step_set S a = ∅ :=
+begin
+  refine Union₂_eq_empty.2 (λ s hs, _),
+  cases s,
+  { exact (hS hs).elim },
+  { simp only [step_char_some, ε_closure_empty] }
+end
+
+-- @[simp] lemma step_set_star [decidable_pred (∈ P.accept)] : P.star.step_set S a = {none} := rfl
+
+@[simp] lemma eval_from_zero_cons (S : set σ) (x : list α) (a : α) :
+  (0 : ε_NFA α σ).eval_from S (a :: x) = ∅ :=
+begin
+  induction x using list.reverse_rec_on,
+  { rw [eval_from_singleton, step_set_zero] },
+  { rw [←list.cons_append, eval_from_append_singleton, step_set_zero] }
+end
+
+@[simp] lemma eval_from_one_cons (S : set σ) (x : list α) (a : α) :
+  (1 : ε_NFA α σ).eval_from S (a :: x) = ∅ :=
+begin
+  induction x using list.reverse_rec_on,
+  { rw [eval_from_singleton, step_set_one] },
+  { rw [←list.cons_append, eval_from_append_singleton, step_set_one] }
+end
+
+-- @[simp] lemma eval_from_add : (P.add Q).accept = {ab | ab.1 ∈ P.accept ∨ ab.2 ∈ Q.accept} := rfl
+-- @[simp] lemma eval_from_mul : (P.mul Q).accept = P.accept ×ˢ Q.accept := rfl
+
+@[simp] lemma eval_from_char [decidable_eq α] (a : α) : (char a).accept = univ := rfl
+
+-- @[simp] lemma eval_from_star [decidable_pred (∈ P.accept)] : P.star.accept = {none} := rfl
+
+@[simp] lemma eval_zero (x : list α) : (0 : ε_NFA α σ).eval x = ∅ := eval_from_empty _ _
+
+@[simp] lemma eval_one_cons (x : list α) (a : α) : (1 : ε_NFA α σ).eval (a :: x) = ∅ :=
+begin
+  induction x using list.reverse_rec_on,
+  { rw [eval_singleton, step_set_one] },
+  { rw [←list.cons_append, eval_append_singleton, step_set_one] }
+end
+
+-- @[simp] lemma eval_add : (P.add Q).accept = {ab | ab.1 ∈ P.accept ∨ ab.2 ∈ Q.accept} := rfl
+-- @[simp] lemma eval_mul : (P.mul Q).accept = P.accept ×ˢ Q.accept := rfl
+
+-- @[simp] lemma eval_char [decidable_eq α] (a : α) : (char a).accept = univ := rfl
+
+-- @[simp] lemma eval_star [decidable_pred (∈ P.accept)] : P.star.accept = {none} := rfl
+
+@[simp] lemma accepts_zero : (0 : ε_NFA α σ).accepts = 0 :=
+eq_empty_of_forall_not_mem $ λ _ ⟨s, h, _⟩, set.not_mem_empty _ h
+
+@[simp] lemma accepts_one [nonempty σ] : (1 : ε_NFA α σ).accepts = 1 :=
 begin
   ext,
   rw language.mem_one,
+  refine ⟨_, λ h, ⟨classical.arbitrary _, mem_univ _, by simp_rw [h, eval_nil, ε_closure_one]⟩⟩,
+  rintro ⟨s, _, hs⟩,
+  cases x,
+  { refl },
+  { rw eval_one_cons at hs,
+    exact hs.elim }
+end
+
+-- @[simp] lemma accepts_add : (P.add Q).accepts = P.accepts + Q.accepts :=
+-- begin
+--   ext,
+--   rw language.mem_add,
+-- end
+
+-- @[simp] lemma accepts_mul : (P.mul Q).accepts = P.accepts * Q.accepts :=
+-- begin
+--   ext,
+--   rw language.mem_mul,
+-- end
+
+@[simp] lemma accepts_char [decidable_eq α] : (char a).accepts = {[a]} :=
+begin
+  ext,
+  rw mem_singleton_iff,
   split,
   {
-    rintro ⟨s, h, hs⟩,
-    sorry,
-  },
-  rintro rfl,
-  sorry
+    rintro ⟨( _ | s), h, hs⟩,
+    cases x,
+    simp at *,
+  }
 end
 
-lemma accepts_add : (P.add Q).accepts = P.accepts + Q.accepts :=
-begin
-  ext,
-  rw language.mem_add,
-end
-
-lemma accepts_mul : (P.mul Q).accepts = P.accepts * Q.accepts :=
-begin
-  ext,
-  rw language.mem_mul,
-end
-
-lemma accepts_star [Π s, decidable (s ∈ P.accept)] : P.star.accepts = P.accepts.star :=
+@[simp] lemma accepts_star [decidable_pred (∈ P.accept)] : P.star.accepts = P.accepts.star :=
 begin
   ext,
   rw language.mem_star,
@@ -167,8 +377,8 @@ begin
 end
 
 lemma pumping_lemma [fintype σ] {x : list α} (hx : x ∈ M.accepts)
-  (hlen : fintype.card (set σ) + 1 ≤ list.length x) :
-  ∃ a b c, x = a ++ b ++ c ∧ a.length + b.length ≤ fintype.card (set σ) + 1 ∧ b ≠ [] ∧
+  (hlen : fintype.card (set σ) ≤ list.length x) :
+  ∃ a b c, x = a ++ b ++ c ∧ a.length + b.length ≤ fintype.card (set σ) ∧ b ≠ [] ∧
   {a} * language.star {b} * {c} ≤ M.accepts :=
 begin
   rw ←to_NFA_correct at hx ⊢,
@@ -189,22 +399,19 @@ def to_ε_NFA (M : NFA α σ) : ε_NFA α σ :=
 @[simp] lemma to_ε_NFA_ε_closure (M : NFA α σ) (S : set σ) : M.to_ε_NFA.ε_closure S = S :=
 begin
   ext a,
-  split,
-  { rintro ( ⟨ _, _, h ⟩ | ⟨ _, _, _, h, _ ⟩ ),
-    exact h,
-    cases h },
-  { intro h,
-    apply ε_NFA.ε_closure.base,
-    exact h }
+  refine ⟨_, ε_NFA.ε_closure.base _⟩,
+  rintro (⟨_, h⟩ | ⟨_, _, h, _⟩),
+  { exact h },
+  { cases h }
 end
 
 @[simp] lemma to_ε_NFA_eval_from_match (M : NFA α σ) (start : set σ) :
   M.to_ε_NFA.eval_from start = M.eval_from start :=
 begin
-  rw [eval_from, ε_NFA.eval_from, step_set, ε_NFA.step_set, to_ε_NFA_ε_closure],
+  rw [eval_from, ε_NFA.eval_from, to_ε_NFA_ε_closure],
   congr,
   ext S s,
-  simp only [exists_prop, set.mem_Union, set.bind_def],
+  simp only [step_set, ε_NFA.step_set, exists_prop, set.mem_Union, set.bind_def],
   apply exists_congr,
   simp only [and.congr_right_iff],
   intros t ht,
